proof/Main.v
@@ -25,6 +25,8 @@ Inductive STEP : exp -> exp -> Prop :=
     ->  STEP  (XApp v1 t2) (XApp v1 t2').
 
 
+Hint Constructors STEP.
+
 
 (* example expressions ************************************)
 Example xId_A := XLam nA tA (XVar nA).
@@ -32,9 +34,6 @@ Example xK_AB := XLam nA tA (XLam nB tB (XVar nA)).
 
 Lemma example_step1 : STEP (XApp xId_A (XAtom nB)) (XAtom nB).
 Proof. unfold xId_A. apply EVAppAbs. auto. Qed.
-
-
-
 
 
 
