proof/TyJudge.v
@@ -1,0 +1,65 @@
+
+Require Import Base.
+Require Import Name.
+Require Import Context.
+Require Import Ty.
+Require Import Exp.
+
+Definition tyenv := partial_map ty.
+
+Inductive TYPE : tyenv -> exp -> ty -> Prop :=
+ | TYVar 
+   :  forall env x T
+   ,  env x = some T
+   -> TYPE env (XVar x) T
+
+ | TYLam 
+   :  forall env x T11 T12 t12
+   ,  TYPE (extend env x T11) t12 T12
+   -> TYPE env                (XLam x T11 t12) (TFun T11 T12)
+
+ | TYApp 
+   :  forall env t1 t2 T11 T12
+   ,  TYPE env t1 (TFun T11 T12)
+   -> TYPE env t2 T11
+   -> TYPE env (XApp t1 t2) T12.
+
+Hint Constructors TYPE.
+
+
+Example type_example1 
+ : TYPE empty (XLam nA tA (XVar nA)) (TFun tA tA).
+Proof. auto. Qed.
+
+
+Example type_example2 
+ : TYPE empty 
+        (XLam nA tA 
+         (XLam nB (TFun tA tA)
+          (XApp (XVar nB) (XApp (XVar nB) (XVar nA)))))
+        (TFun tA (TFun (TFun tA tA) tA)).
+Proof.
+ apply TYLam.  apply TYLam.
+ eapply TYApp. apply TYVar. apply extend_eq. 
+ eapply TYApp. apply TYVar. apply extend_eq. 
+ eapply TYVar. unfold extend. simpl. tauto.
+Qed.
+
+
+Example type_nonexample1
+ : ~exists T 
+ , TYPE empty 
+        (XLam nA tA
+         (XLam nB tB
+          (XApp (XVar nA) (XVar nB))))
+        T.
+Proof. 
+ intros C. destruct C.
+ inversion H.  subst. clear H.
+ inversion H5. subst. clear H5.
+ inversion H4. subst. clear H4.
+ inversion H2. subst. clear H2.
+ inversion H5. subst. clear H5.
+ unfold extend in H1. simpl in H1.
+ inversion H1.
+Qed.
